Matroid/Constructions/ParallelExtension.lean
@@ -1,0 +1,438 @@
+import Matroid.Simple
+import Matroid.Closure
+import Matroid.Minor.Basic
+import Matroid.Map
+import Matroid.ForMathlib.Other
+
+open Set Function Set.Notation
+namespace Matroid
+
+
+
+section Set
+
+/-- Replace the elements of `S` with parallel copies of `e`. -/
+def parallelExtendSet {α : Type*} (M : Matroid α) (e : α) (S : Set α) [DecidablePred (· ∈ S)] :
+    Matroid α :=
+  M.comap (fun x ↦ if (x ∈ S) then e else x)
+
+end Set
+
+
+section Loop
+
+variable {α : Type*} {M M' : Matroid α} {e f : α} {I : Set α}
+
+/-- Add a loop `e` to a matroid `M`. Has the junk value `M` if `e ∈ M.E` -/
+def addLoop (M : Matroid α) (e : α) : Matroid α := M ↾ (insert e M.E)
+
+lemma addLoop_eq_self (he : e ∈ M.E) : M.addLoop e = M := by
+  rw [addLoop, insert_eq_of_mem he, restrict_ground_eq_self]
+
+@[simp] lemma addLoop_ground (M : Matroid α) (e : α) : (M.addLoop e).E = insert e M.E := rfl
+
+@[simp] lemma addLoop_indep_iff : (M.addLoop f).Indep I ↔ M.Indep I := by
+  simp only [addLoop, restrict_indep_iff, and_iff_left_iff_imp]
+  exact fun hI ↦ hI.subset_ground.trans (subset_insert _ _)
+
+lemma eq_addLoop_iff (he : e ∉ M.E) : M' = M.addLoop e ↔ M'.Loop e ∧ M' ＼ e = M := by
+  obtain (he' | he') := em' (e ∈ M'.E)
+  · refine iff_of_false ?_ ?_
+    · rintro rfl; simp at he'
+    rintro ⟨h, rfl⟩; exact he' h.mem_ground
+
+  simp_rw [deleteElem, eq_iff_indep_iff_indep_forall, addLoop_ground, addLoop_indep_iff,
+    delete_ground, delete_indep_iff, disjoint_singleton_right, ← singleton_dep, dep_iff,
+    singleton_subset_iff, and_iff_left he', subset_diff, disjoint_singleton_right, and_imp]
+
+  refine ⟨fun ⟨hE, hi⟩ ↦ ⟨?_, ?_, ?_⟩, fun ⟨hi, hE, h⟩ ↦ ⟨?_, fun I hIss ↦ ?_⟩⟩
+  · rw [hi _ (singleton_subset_iff.2 he')]
+    exact fun hei ↦ he (singleton_subset_iff.1 hei.subset_ground)
+  · simp [hE, he]
+  · rintro I hIss heI
+    rw [and_iff_left heI, hi _ hIss]
+  · rw [← hE, insert_diff_singleton, insert_eq_of_mem he']
+  obtain (heI | heI) := em (e ∈ I)
+  · exact iff_of_false (fun hI ↦ hi <| hI.subset (singleton_subset_iff.2 heI))
+      (fun hI ↦ he <| hI.subset_ground heI)
+  specialize h I hIss
+  simpa [heI] using h
+
+lemma addLoop_loop (he : e ∉ M.E) : (M.addLoop e).Loop e := by
+  rw [addLoop, ← singleton_dep, Dep, singleton_subset_iff, restrict_indep_iff,
+    singleton_subset_iff, restrict_ground_eq, and_iff_left (mem_insert _ _),
+    and_iff_left (mem_insert _ _)]
+  exact fun hi ↦ he (singleton_subset_iff.1 hi.subset_ground)
+
+instance addLoop_finite (M : Matroid α) [M.Finite] (e : α) : (M.addLoop e).Finite :=
+  ⟨M.ground_finite.insert e⟩
+
+instance addLoop_finiteRk (M : Matroid α) [M.FiniteRk] (e : α) : (M.addLoop e).FiniteRk := by
+  obtain ⟨B, hB⟩ := (addLoop M e).exists_base
+  exact ⟨⟨B, hB, (addLoop_indep_iff.1 hB.indep).finite⟩⟩
+
+instance addLoop_finitary (M : Matroid α) [M.Finitary] (e : α) : (M.addLoop e).Finitary := by
+  refine ⟨fun I hI ↦ ?_⟩
+  simp only [addLoop_indep_iff] at *
+  exact Finitary.indep_of_forall_finite I hI
+
+def addColoop (M : Matroid α) (e : α) : Matroid α := (M✶.addLoop e)✶
+
+lemma addColoop_eq_self (he : e ∈ M.E) : M.addColoop e = M := by
+  rwa [addColoop, addLoop_eq_self, dual_dual]
+
+@[simp] lemma addColoop_ground (M : Matroid α) (e : α) : (M.addColoop e).E = insert e M.E := rfl
+
+lemma eq_addColoop_iff (he : e ∉ M.E) : M' = M.addColoop e ↔ M'.Coloop e ∧ (M' ／ e) = M := by
+  rw [addColoop, eq_dual_comm, eq_comm, eq_addLoop_iff (show e ∉ M✶.E from he),
+    dual_loop_iff_coloop, eq_dual_comm, deleteElem, dual_delete_dual_eq_contract, contract_elem,
+    eq_comm]
+
+end Loop
+
+section Parallel
+
+variable {α : Type*} [DecidableEq α] {M M' : Matroid α} {e f x : α} {I C : Set α}
+
+/-- Replace `f` with a parallel copy of `e` in `M`. Intended for use where `e` is a nonloop
+  and `f ∉ M.E`. When this is not the case, the junk value is described by
+  either `parallelExtend_not_nonloop` or `parallelExtend_delete_eq` -/
+def parallelExtend (M : Matroid α) (e f : α) : Matroid α :=
+  (M.comap (update id f e)) ↾ (insert f M.E)
+
+@[simp] lemma parallelExtend_ground (M : Matroid α) (e f : α) :
+    (M.parallelExtend e f).E = insert f M.E := rfl
+
+@[simp] lemma parallelExtend_self (M : Matroid α) (e : α) :
+    M.parallelExtend e e = M.addLoop e := by
+  change comap _ (update id e (id e)) ↾ _ = _
+  rw [update_eq_self, comap_id, addLoop]
+
+lemma parallelExtend_not_nonloop (he : ¬M.Nonloop e) (f : α) :
+    M.parallelExtend e f = (M ＼ f).addLoop f := by
+  classical
+  simp only [parallelExtend, deleteElem, eq_iff_indep_iff_indep_forall, restrict_ground_eq,
+    addLoop_ground, delete_ground, mem_diff, mem_singleton_iff, not_true_eq_false, and_false,
+    insert_diff_singleton, restrict_indep_iff, comap_indep_iff, ne_eq, image_update, id_eq,
+    image_id', update_id_injOn_iff, addLoop_indep_iff, delete_indep_iff, disjoint_singleton_right,
+    true_and]
+
+  rintro I hI
+  split_ifs with hf
+  · simp [(show ¬ M.Indep (insert e _) from fun hi ↦ he <| hi.nonloop_of_mem (mem_insert _ _)), hf]
+  simp [hf, hI]
+
+lemma parallelExtend_eq_parallelExtend_delete (M : Matroid α) {e f : α} (hef : e ≠ f):
+    M.parallelExtend e f = (M ＼ f).parallelExtend e f := by
+  classical
+  rw [parallelExtend, parallelExtend, deleteElem, delete_ground, insert_diff_singleton,
+    eq_iff_indep_iff_indep_forall]
+  simp only [restrict_ground_eq, restrict_indep_iff, comap_indep_iff, ne_eq, image_update, id_eq,
+    image_id', mem_diff, mem_singleton_iff, update_id_injOn_iff, delete_indep_iff,
+    disjoint_singleton_right, and_congr_left_iff, iff_self_and, true_and]
+  aesop
+
+/-- Deleting `f` in a parallel extension of `M` by `f` is the same as deleting `f` from `M`.
+  This could be a simp lemma, but it is less convenient than the 'non-junk' unprimed version,
+  which is simpler for reasonable inputs, even though it requires `f ∉ M.E` explicitly.  -/
+lemma parallelExtend_delete_eq' (M : Matroid α) (e f : α) :
+    (M.parallelExtend e f) ＼ f = M ＼ f := by
+  classical
+  simp only [parallelExtend, deleteElem, eq_iff_indep_iff_indep_forall, delete_ground,
+    restrict_ground_eq, mem_insert_iff, true_or, not_true_eq_false, mem_singleton_iff,
+    insert_diff_of_mem, subset_diff, disjoint_singleton_right, delete_indep_iff, restrict_indep_iff,
+    comap_indep_iff, ne_eq, image_update, id_eq, image_id', mem_diff, update_id_injOn_iff,
+    and_congr_left_iff, and_imp, true_and]
+  rintro I - hf -
+  simp only [hf, not_false_eq_true, diff_singleton_eq_self, ite_false, IsEmpty.forall_iff, and_true,
+    and_iff_left_iff_imp]
+  exact fun hI ↦ hI.subset_ground.trans <| subset_insert _ _
+
+lemma parallelExtend_delete_eq (e : α) (hf : f ∉ M.E) : (M.parallelExtend e f) ＼ f = M := by
+  rwa [parallelExtend_delete_eq', deleteElem, delete_eq_self_iff, disjoint_singleton_left]
+
+lemma parallelExtend_nonloop_iff (he : M.Nonloop e) :
+    (M.parallelExtend e f).Nonloop x ↔ M.Nonloop x ∨ x = f := by
+  classical
+  rw [← indep_singleton, parallelExtend, restrict_indep_iff, singleton_subset_iff,
+    comap_indep_iff, and_iff_left (injOn_singleton _ _), mem_insert_iff,
+    image_update, image_id, image_id]
+  obtain (rfl | hne) := eq_or_ne x f
+  · simpa
+  simp only [mem_singleton_iff, hne.symm, not_false_eq_true, diff_singleton_eq_self, ite_false,
+    indep_singleton, hne, false_or, or_false, and_iff_left_iff_imp]
+  exact Nonloop.mem_ground
+
+lemma parallelExtend_parallel (he : M.Nonloop e) (f : α) : (M.parallelExtend e f).Parallel e f := by
+  classical
+  have he' : (M.parallelExtend e f).Nonloop e := by
+    rw [parallelExtend_nonloop_iff he]; left; assumption
+  have hf : (M.parallelExtend e f).Nonloop f := by
+    rw [parallelExtend_nonloop_iff he]; right; rfl
+  obtain (rfl | hef) := eq_or_ne e f
+  · rwa [parallel_self_iff]
+  rw [he'.parallel_iff_dep hf hef, Dep, pair_subset_iff, and_iff_right he'.mem_ground,
+    and_iff_left hf.mem_ground, parallelExtend, restrict_indep_iff, comap_indep_iff,
+    image_update, image_id, image_id,
+    if_pos (mem_insert_of_mem _ (show f ∈ ({f} : Set α) from rfl))]
+  exact fun hcon ↦ hef <| hcon.1.2 (by simp) (by simp) (by simp [update_noteq hef e id])
+
+lemma eq_parallelExtend_iff (he : M.Nonloop e) (hf : f ∉ M.E) :
+    M' = M.parallelExtend e f ↔ M'.Parallel e f ∧ M' ＼ f = M := by
+  classical
+  constructor
+  · rintro rfl; exact ⟨parallelExtend_parallel he f, parallelExtend_delete_eq e hf⟩
+  rintro ⟨h, rfl⟩
+  simp only [deleteElem, delete_nonloop_iff, mem_singleton_iff] at he
+  refine eq_of_indep_iff_indep_forall (by simp [insert_eq_of_mem h.mem_ground_right])
+    (fun I hI ↦ ?_)
+  obtain (hfI | hfI) := em' (f ∈ I)
+  · simp [hfI, parallelExtend, hI.trans (subset_insert _ _)]
+  suffices M'.Indep I ↔ M'.Indep (insert e (I \ {f})) ∧ e ∉ I by
+    simpa [hfI, parallelExtend, Ne.symm he.2, hI.trans (subset_insert _ _)]
+  obtain (heI | heI) := em (e ∈ I)
+  · simp [heI, show ¬ M'.Indep I from
+      fun hI ↦ he.2 (h.eq_of_indep (hI.subset (pair_subset heI hfI)))]
+  simp [heI, h.parallel'.symm.indep_substitute_iff hfI heI]
+
+lemma parallelExtend_cl_eq_of_mem (he : M.Nonloop e) (hf : f ∉ M.E) (X : Set α)
+    (heX : e ∈ M.cl X) : (M.parallelExtend e f).cl X = insert f (M.cl X) := by
+  nth_rw 2 [← M.parallelExtend_delete_eq e hf]
+  simp only [deleteElem, delete_cl_eq, insert_diff_singleton]
+  rw [← M.parallelExtend_delete_eq e hf, deleteElem, delete_cl_eq, mem_diff,
+    (parallelExtend_parallel he f).mem_cl_iff_mem_cl] at heX
+  rw [cl_diff_singleton_eq_cl heX.1, eq_comm, insert_eq_self]
+  exact mem_of_mem_of_subset heX.1 (cl_subset_cl _ (diff_subset _ _))
+
+lemma parallelExtend_cl_eq_of_not_mem_not_mem (he : M.Nonloop e) (hf : f ∉ M.E) {X : Set α}
+    (heX : e ∉ M.cl X) (hfX : f ∉ X) : (M.parallelExtend e f).cl X = M.cl X := by
+  nth_rw 2 [← M.parallelExtend_delete_eq e hf]
+  have hfX' : f ∉ (M.parallelExtend e f).cl (X \ {f}) := by
+    rw [← M.parallelExtend_delete_eq e hf, deleteElem, delete_cl_eq, mem_diff,
+      (parallelExtend_parallel he f).mem_cl_iff_mem_cl] at heX
+    simpa [(show e ≠ f by rintro rfl; exact hf he.mem_ground)] using heX
+  simp only [deleteElem, delete_cl_eq, diff_singleton_eq_self hfX']
+  rw [diff_singleton_eq_self hfX]
+
+-- lemma foo (he : M.Nonloop e) (hf : f ∉ M.E) (X : Set α) {heX : e ∉ M.cl X} :
+--     (M.parallelExtend e f).cl X = (X ∩ {f}) ∪ M.cl (X \ {f}) := by
+--   nth_rw 2 [← M.parallelExtend_delete_eq e hf]
+--   have hfX' : f ∉ (M.parallelExtend e f).cl (X \ {f}) := by
+--     rw [← M.parallelExtend_delete_eq e hf, deleteElem, delete_cl_eq, mem_diff,
+--       (parallelExtend_parallel he f).mem_cl_iff_mem_cl] at heX
+--     simpa [(show e ≠ f by rintro rfl; exact hf he.mem_ground)] using heX
+--   obtain (hf | hf) := em (f ∈ X)
+--   · rw [inter_eq_self_of_subset_right (by simpa), singleton_union]
+--     simp only [deleteElem, delete_cl_eq, sdiff_idem, insert_diff_singleton]
+--     refine subset_antisymm ?_ ?_
+--     ·
+--   rw [inter_singleton_eq_empty.2 hf, empty_union, deleteElem, delete_cl_eq, diff_diff,
+--     union_self, diff_singleton_eq_self hf, diff_singleton_eq_self]
+--   rwa [← diff_singleton_eq_self hf]
+
+
+-- lemma parallelExtend_cl_eq_of_not_mem_mem (he : M.Nonloop e) (hf : f ∉ M.E) (X : Set α)
+--     (heX : e ∉ M.cl X) (hfX : f ∈ X) :
+--     (M.parallelExtend e f).cl X = insert f (M.cl (insert e (X \ {f}))) := by
+--   nth_rw 2 [← M.parallelExtend_delete_eq e hf]
+--   simp only [deleteElem, delete_cl_eq, sdiff_idem, insert_diff_singleton]
+--   rw [← M.parallelExtend_delete_eq e hf] at heX
+
+--   simp [(show e ≠ f by rintro rfl; exact hf he.mem_ground),
+--     (parallelExtend_parallel he f).mem_cl_iff_mem_cl] at heX
+--   ext x
+--   ·
+    -- simp only [deleteElem, delete_cl_eq, mem_diff, mem_single
+
+lemma parallelExtend_indep_iff (he : M.Nonloop e) (hf : f ∉ M.E) :
+    (M.parallelExtend e f).Indep I ↔
+      (f ∉ I ∧ M.Indep I) ∨ (f ∈ I ∧ e ∉ I ∧ M.Indep (insert e (I \ {f}))) := by
+
+
+lemma parallelExtend_indep_iff (he : M.Nonloop e) (hf : f ∉ M.E) :
+    (M.parallelExtend e f).Indep I ↔
+      (f ∉ I ∧ M.Indep I) ∨ (f ∈ I ∧ e ∉ I ∧ M.Indep (insert e (I \ {f}))) := by
+  have hdel : ∀ J, f ∉ J → ((M.parallelExtend e f).Indep J ↔ M.Indep J) := by
+    rintro J hfJ
+    convert (delete_indep_iff (M := M.parallelExtend e f) (D := {f}) (I := J)).symm using 1
+    · rw [disjoint_singleton_right, and_iff_left hfJ]
+    rw [← deleteElem, parallelExtend_delete_eq', deleteElem, delete_indep_iff,
+      disjoint_singleton_right, and_iff_left hfJ]
+  have hef : e ≠ f := by rintro rfl; exact hf he.mem_ground
+
+  obtain (hfI | hfI) := em (f ∈ I)
+  · rw [iff_true_intro hfI, not_true, false_and, false_or, true_and]
+    obtain (heI | heI) := em (e ∈ I)
+    · simp only [heI, not_true_eq_false, mem_diff, mem_singleton_iff, true_and, false_and,
+        iff_false, parallelExtend_ground]
+      exact fun hi ↦ ((parallelExtend_parallel he f).dep_of_ne hef).not_indep
+        (hi.subset (pair_subset heI hfI))
+    rw [and_iff_right heI,
+      (parallelExtend_parallel he f).parallel'.symm.indep_substitute_iff hfI heI, hdel]
+    rintro (rfl | h); exact hef rfl
+    exact h.2 rfl
+
+  simp [hdel _ hfI, hfI]
+
+
+lemma parallelExtend_circuit_iff (he : M.Nonloop e) (hf : f ∉ M.E) :
+    (M.parallelExtend e f).Circuit C ↔ M.Circuit C ∨ C = {e,f} ∨
+        f ∈ C ∧ e ∉ C ∧ M.Circuit (insert e (C \ {f})) := by
+  have hef : e ≠ f := by rintro rfl; exact hf he.mem_ground
+  simp only [circuit_iff_dep_forall_diff_singleton_indep, parallelExtend_indep_iff he hf, mem_diff,
+    dep_iff, mem_singleton_iff, not_and, Decidable.not_not, mem_insert_iff, forall_eq_or_imp,
+    insert_diff_of_mem, and_imp]
+  obtain (hfC | hfC) := em' (f ∈ C)
+  · have hne : C ≠ {e,f} := by rintro rfl; exact hfC (.inr rfl)
+    simp [hfC, hne, subset_insert_iff]
+  simp only [hfC, not_true_eq_false, false_and, true_and, false_or, not_and, parallelExtend_ground,
+    true_implies]
+  obtain (heC | heC) := em (e ∈ C)
+  · simp only [heC, not_true_eq_false, false_implies, true_and, true_implies,
+      show ¬C ⊆ M.E from sorry, and_false, false_and, or_false, false_or]
+
+
+
+
+  -- simp only [circuit_iff_dep_forall_diff_singleton_indep, dep_iff, parallelExtend_indep_iff he hf,
+  --   not_or, not_and, parallelExtend_ground, mem_diff, mem_singleton_iff, Decidable.not_not,
+  --   mem_insert_iff, forall_eq_or_imp, insert_diff_of_mem, and_imp]
+  -- obtain (hfC | hfC) := em' (f ∈ C)
+  -- · rw [circuit_iff_delete_of_disjoint (disjoint_singleton_right.2 hfC), ← deleteElem,
+  --     parallelExtend_delete_eq _ hf, iff_false_intro hfC, false_and, or_false, or_iff_left]
+  --   rintro rfl
+  --   simp at hfC
+  -- refine ⟨fun h ↦ ?_, fun h ↦ ?_⟩
+  -- · sorry
+  -- sorry
+
+  -- obtain (hfC | hfC) := em' (f ∈ C)
+  -- · rw [circuit_iff_delete_of_disjoint (disjoint_singleton_right.2 hfC), ← deleteElem,
+  --     parallelExtend_delete_eq _ hf, iff_false_intro hfC, false_and, or_false, or_iff_left]
+  --   rintro rfl
+  --   simp at hfC
+  -- set i := isoOfSwapParallel (parallelExtend_parallel he f).parallel' with hi_def
+  -- obtain (hss | hnss) := em (C ⊆ (parallelExtend M e f).E)
+  -- · have hnC : ¬ M.Circuit C := fun hC ↦ hf (hC.subset_ground hfC)
+  --   rw [or_iff_right hnC, and_iff_right hfC]
+  --   by_cases heC : e ∈ C
+  --   · rw [iff_true_intro heC, not_true, false_and, or_false]
+  --     have hC := (parallelExtend_parallel he f).circuit_of_ne hef
+  --     exact ⟨fun h ↦ (hC.eq_of_subset_circuit h (pair_subset heC hfC)).symm, fun h ↦ by rwa [h]⟩
+  --   have hfC' : f ∉ i '' (M.E ↓∩ C) := by simpa [hi_def]
+  --   rw [or_iff_right (show C ≠ {e,f} by rintro rfl; exact heC (Or.inl rfl)), and_iff_right heC,
+  --     i.on_circuit_iff, circuit_iff_delete_of_disjoint (disjoint_singleton_right.2 hfC'),
+  --     ← deleteElem, parallelExtend_delete_eq _ hf, parallel_swap_apply, parallelExtend_ground,
+  --     PartialEquiv.restr_coe, Equiv.toPartialEquiv_apply, Equiv.swap_comm,
+  --     Equiv.swap_image_eq_exchange hfC heC]
+
+  -- refine iff_of_false (fun hC ↦ hnss hC.subset_ground) ?_
+  -- rw [parallelExtend_ground] at hnss
+  -- rintro (hC | rfl | hC)
+  -- · exact hnss (hC.subset_ground.trans (subset_insert _ _))
+  -- · exact hnss (pair_subset (mem_insert_of_mem _ he.mem_ground) (mem_insert _ _))
+  -- have hss := hC.2.2.subset_ground
+  -- rw [insert_subset_iff, diff_subset_iff, singleton_union] at hss
+  -- exact hnss hss.2
+
+instance parallelExtend_finite (M : Matroid α) [M.Finite] (e f : α) :
+    (M.parallelExtend e f).Finite :=
+  ⟨M.ground_finite.insert f⟩
+
+instance parallelExtend_finiteRk (M : Matroid α) [FiniteRk M] (e f : α) :
+    (M.parallelExtend e f).FiniteRk := by
+  obtain ⟨B, hB⟩ := (M.parallelExtend e f).exists_base
+  have hB' : M.Indep (B \ {f}) := by
+    rw [indep_iff_delete_of_disjoint (disjoint_sdiff_left (t := B) (s := {f})),
+      ← deleteElem, ← parallelExtend_delete_eq' M e f, deleteElem, delete_indep_iff,
+      and_iff_left disjoint_sdiff_left]
+    exact hB.indep.subset <| diff_subset _ _
+  exact ⟨⟨_, hB, (hB'.finite.insert f).subset <| by simp⟩⟩
+
+instance parallelExtend_finitary (M : Matroid α) [Finitary M] (e f : α) :
+    (M.parallelExtend e f).Finitary := by
+  obtain (rfl | hef) := eq_or_ne e f
+  · rw [parallelExtend_self]; infer_instance
+  obtain (he | he) := em' (M.Nonloop e)
+  · rw [parallelExtend_not_nonloop he]
+    infer_instance
+  rw [parallelExtend_eq_parallelExtend_delete _ hef, finitary_iff_forall_circuit_finite]
+  intro C
+  rw [parallelExtend_circuit_iff, deleteElem, delete_circuit_iff, disjoint_singleton_right,
+    delete_circuit_iff]
+  · rintro (h | rfl | h)
+    · exact h.1.finite
+    · exact toFinite {e, f}
+    refine (h.2.2.1.finite.insert f).subset ?_
+    rw [insert_comm, insert_diff_singleton]
+    exact (subset_insert _ _).trans (subset_insert _ _)
+  · rwa [deleteElem, delete_nonloop_iff, and_iff_right he]
+  exact fun h ↦ h.2 rfl
+
+end Parallel
+
+section Series
+
+variable {α : Type*} [DecidableEq α] {M M' : Matroid α} {e f : α}
+
+/-- Coextend `e` by `f` in series. Intended for use where `e` is a non-coloop and `f ∉ M.E`. -/
+def seriesExtend (M : Matroid α) (e f : α) : Matroid α := (M✶.parallelExtend e f)✶
+
+@[simp] lemma seriesExtend_dual (M : Matroid α) (e f : α) :
+    (M.seriesExtend e f)✶ = M✶.parallelExtend e f := by
+  rw [seriesExtend, dual_dual]
+
+@[simp] lemma parallelExtend_dual (M : Matroid α) (e f : α) :
+    (M.parallelExtend e f)✶ = M✶.seriesExtend e f := by
+  rw [seriesExtend, dual_dual]
+
+@[simp] lemma seriesExtend_ground (M : Matroid α) (e f : α) :
+    (M.seriesExtend e f).E = insert f M.E := rfl
+
+@[simp] lemma seriesExtend_self (M : Matroid α) (e : α) :
+    M.seriesExtend e e = M.addColoop e := by
+  rw [seriesExtend, parallelExtend_self, addColoop]
+
+lemma seriesExtend_coloop (he : M.Coloop e) (f : α) :
+    M.seriesExtend e f = (M ／ f).addColoop f := by
+  rw [seriesExtend, parallelExtend_not_nonloop, addColoop, deleteElem, contract_elem,
+    contract_dual_eq_dual_delete]
+  simp [Nonloop, dual_loop_iff_coloop, he]
+
+lemma seriesExtend_not_mem_ground (he : e ∉ M.E) (f : α) :
+    M.seriesExtend e f = (M ／ f).addColoop f := by
+  rw [seriesExtend, parallelExtend_not_nonloop, addColoop, contract_elem, deleteElem,
+    contract_dual_eq_dual_delete]
+  simp [Nonloop, he]
+
+lemma seriesExtend_eq_seriesExtend_contract (M : Matroid α) {e f : α} (hef : e ≠ f):
+    M.seriesExtend e f = (M ／ f).seriesExtend e f := by
+  rw [seriesExtend, parallelExtend_eq_parallelExtend_delete _ hef, seriesExtend]
+  simp only [deleteElem, contract_elem, contract_dual_eq_dual_delete]
+
+lemma seriesExtend_contract_eq' (M : Matroid α) (e f : α) :
+    ((M.seriesExtend e f) ／ f) = M ／ f := by
+  rw [seriesExtend, contract_elem, ← delete_dual_eq_dual_contract, ← deleteElem,
+    parallelExtend_delete_eq']
+  simp
+
+lemma seriesExtend_contract_eq (e : α) (hf : f ∉ M.E) : (M.seriesExtend e f ／ f) = M := by
+  rw [seriesExtend, contract_elem, ← delete_dual_eq_dual_contract, ← deleteElem,
+    parallelExtend_delete_eq _ (show f ∉ M✶.E from hf), dual_dual]
+
+lemma seriesExtend_series (heE : e ∈ M.E) (he : ¬M.Coloop e) (f : α) :
+    (M.seriesExtend e f).Series e f := by
+  rw [Series, seriesExtend, dual_dual]
+  apply parallelExtend_parallel
+  rwa [Nonloop, dual_ground, and_iff_left heE, dual_loop_iff_coloop]
+
+lemma eq_seriesExtend_iff (heE : e ∈ M.E) (he : ¬M.Coloop e) (hf : f ∉ M.E) :
+    M' = M.seriesExtend e f ↔ M'.Series e f ∧ ((M' ／ f) = M) := by
+  rw [seriesExtend, eq_dual_comm, eq_comm, eq_parallelExtend_iff _ (show f ∉ M✶.E from hf),
+    deleteElem, ← contract_dual_eq_dual_delete, ← contract_elem, dual_inj, Series]
+  rwa [Nonloop, and_iff_left (show e ∈ M✶.E from heE), dual_loop_iff_coloop]
+
+instance seriesExtend_finite (M : Matroid α) [M.Finite] : (M.seriesExtend e f).Finite :=
+  ⟨M.ground_finite.insert f⟩
+
+end Series
